Capless/Subst/Capture/Typing.lean
@@ -7,4 +7,8 @@ theorem Typed.csubst
   (σ : CVarSubst Γ f Δ) :
   Typed Δ (t.crename f) (E.crename f) := by sorry
 
+theorem Typed.copen
+  (h : Typed (Γ.cvar CBinding.bound) t E) :
+  Typed Γ (t.copen c) (E.copen c) := by sorry
+
 end Capless
